@prefix ppb: <http://parliament.uk/ontologies/parliamentary-bloc/> . 
@prefix xsd: <http://www.w3.org/2001/XMLSchema#> . 
@prefix rdf: <http://www.w3.org/1999/02/22-rdf-syntax-ns#> .
@prefix dcterms: <http://purl.org/dc/terms/> .
@prefix owl:     <http://www.w3.org/2002/07/owl#> .
@prefix rdfs:    <http://www.w3.org/2000/01/rdf-schema#> .
@prefix foaf:	<http://xmlns.com/foaf/0.1/> .

<http://parliament.uk/ontologies/parliamentary-bloc/> 
    rdf:type owl:Ontology ;
    dcterms:title "Parliamentary bloc ontology"@en ;
    dcterms:created "2017-06-14"^^xsd:date ;
	dcterms:rights "Open Parliament Licence v3.0"@en ;
    dcterms:description "The parliamentary bloc ontology for UK Parliament extends and specialises the agency model to describe whippings to parliamentary parties and affiliations to parliamentary blocs."@en ;
	foaf:depiction <https://ukparliament.github.io/ontologies/parliamentary-bloc/parliamentary-bloc.png> ;
	foaf:maker
		[ foaf:name "David Beamish" ],
		[ foaf:name "Robert Brook"; foaf:homepage <https://robert-brook.com/> ],
		[ foaf:name "Oli Hawkins"; foaf:homepage <https://olihawkins.com/> ],
		[ foaf:name "Lucinda Maer" ],
		[ foaf:name "Silver Oliver" ],
		[ foaf:name "Michael Smethurst"; foaf:homepage <http://smethur.st/> ],
	    [ foaf:name "Anya Somerville" ].


#######  Classes ##### 	

ppb:Pact rdf:type owl:Class ;
	rdfs:label "Pact"@en ;
	rdfs:comment "An agreement between two or more political parties."@en ;
	rdfs:isDefinedBy <http://parliament.uk/ontologies/parliamentary-bloc/> .
	
ppb:Sistership rdf:type owl:Class ;
	rdfs:label "Sistership"@en ;
	rdfs:comment "A relationship between political parties who have agreed to co-operate."@en ;
	rdfs:isDefinedBy <http://parliament.uk/ontologies/parliamentary-bloc/> .
	
ppb:ParliamentaryAgreement rdf:type owl:Class ;
	rdfs:label "Parliamentary agreement"@en ;
	rdfs:comment "An agreement between two or more parliamentary parties to cooperate within Parliament, for example: a confidence and supply or coalition agreement."@en ;
	rdfs:isDefinedBy <http://parliament.uk/ontologies/parliamentary-bloc/> .
	
ppb:PoliticalParty rdf:type owl:Class ;
	rdfs:label "Political party"@en ;
	rdfs:comment "A group registered with the Electoral Commission as a political party."@en ;
	rdfs:isDefinedBy <http://parliament.uk/ontologies/parliamentary-bloc/> .
	
ppb:ParliamentaryParty rdf:type owl:Class ;
	rdfs:subClassOf ppb:ParliamentaryBloc ;
	rdfs:label "Parliamentary party"@en ;
	rdfs:comment "A group of Members of Parliament accepting a party whip."@en ;
	rdfs:isDefinedBy <http://parliament.uk/ontologies/parliamentary-bloc/> .
	
ppb:ParliamentaryBloc rdf:type owl:Class ;
	rdfs:label "Parliamentary bloc"@en ;
	rdfs:comment "A group of Members of Parliament named for the purposes of administration, for example: a parliamentary party, the bishops or Crossbenchers in the House of Lords."@en ;
	rdfs:isDefinedBy <http://parliament.uk/ontologies/parliamentary-bloc/> .
	
ppb:Affiliation rdf:type owl:Class ;
	rdfs:label "Affiliation"@en ;
	rdfs:comment "An affiliation to a parliamentary bloc held by a Member between two dates, for example: an affiliation to the Co-operative Party whilst accepting the whip of the Labour Party."@en ;
	rdfs:isDefinedBy <http://parliament.uk/ontologies/parliamentary-bloc/> .
	
ppb:MemberWhipping rdf:type owl:Class ;
	rdfs:subClassOf ppb:Affiliation ;
	rdfs:label "Member whipping"@en ;
	rdfs:comment "The acceptance of a whip to a parliamentary party by a Member between two dates: the whip may be withdrawn by a party or declined by a Member."@en ;
	rdfs:isDefinedBy <http://parliament.uk/ontologies/parliamentary-bloc/> .
	
ppb:Member rdf:type owl:Class ;
	rdfs:label "Member"@en ;
	rdfs:comment "A person who is or has been a Member of Parliament."@en ;
	rdfs:isDefinedBy <http://parliament.uk/ontologies/parliamentary-bloc/> .
	

	
##### Object properties ####


ppb:hasPact rdf:type owl:ObjectProperty ;
	rdfs:label "Has pact"@en ;
	rdfs:comment "The relationship between a political party and the inclusion of that party within a pact."@en ;
	rdfs:domain ppb:PoliticalParty ;
	rdfs:range ppb:Pact ;
	rdfs:isDefinedBy <http://parliament.uk/ontologies/parliamentary-bloc/> .
	
ppb:hasSistership rdf:type owl:ObjectProperty ;
	rdfs:label "Has sistership"@en ;
	rdfs:comment "The relationship between a political party and the participation of that party within a sistership."@en ;
	rdfs:domain ppb:PoliticalParty ;
	rdfs:range ppb:Sistership ;
	rdfs:isDefinedBy <http://parliament.uk/ontologies/parliamentary-bloc/> .
	
ppb:hasParliamentaryAgreement rdf:type owl:ObjectProperty ;
	rdfs:label "Has parliamentary agreement"@en ;
	rdfs:comment "The relationship between a parliamentary party and the participation of that party in an agreement."@en ;
	rdfs:domain ppb:ParliamentaryParty ;
	rdfs:range ppb:ParliamentaryAgreement ;
	rdfs:isDefinedBy <http://parliament.uk/ontologies/parliamentary-bloc/> .
	
ppb:hasAssociation rdf:type owl:ObjectProperty ;
	rdfs:label "Has association"@en ;
	rdfs:comment "The relationship between a party within Parliament and the membership of the party outside Parliament."@en ;
	rdfs:domain ppb:ParliamentaryParty ;
	rdfs:range ppb:PoliticalParty ;
	rdfs:isDefinedBy <http://parliament.uk/ontologies/parliamentary-bloc/> .
	
ppb:hasAffiliation rdf:type owl:ObjectProperty ;
	rdfs:label "Has affiliation"@en ;
	rdfs:comment "The relationship between an affiliation of a Member and a parliamentary bloc, for example: between a affiliation of a Crossbencher and the Crossbenchers in the House of Lords."@en ;
	rdfs:domain ppb:ParliamentaryBloc ;
	rdfs:range ppb:Affiliation ;
	rdfs:isDefinedBy <http://parliament.uk/ontologies/parliamentary-bloc/> .
	
ppb:whippedTo rdf:type owl:ObjectProperty ;
	rdfs:label "Whipped to"@en ;
	rdfs:comment "The relationship between a whipping of a Member and a parliamentary party, for example: between the whipping of a Liberal Member and the parliamentary Liberal Party."@en ;
	rdfs:domain ppb:MemberWhipping ;
	rdfs:range ppb:ParliamentaryParty ;
	rdfs:isDefinedBy <http://parliament.uk/ontologies/parliamentary-bloc/> .
	
ppb:accepts rdf:type owl:ObjectProperty ;
	rdfs:label "Accepts"@en ;
	rdfs:comment "The relationship between a Member and a whipping of that Member: the acceptance of a whip by a Member."@en ;
	rdfs:domain ppb:Member ;
	rdfs:range ppb:MemberWhipping ;
	rdfs:isDefinedBy <http://parliament.uk/ontologies/parliamentary-bloc/> .
				
	
##### Data properties ####	
			

						