@prefix ppr: <http://parliament.uk/ontologies/procedure/> . 
@prefix xsd: <http://www.w3.org/2001/XMLSchema#> . 
@prefix rdf: <http://www.w3.org/1999/02/22-rdf-syntax-ns#> .
@prefix dcterms: <http://purl.org/dc/terms/> .
@prefix owl:     <http://www.w3.org/2002/07/owl#> .
@prefix rdfs:    <http://www.w3.org/2000/01/rdf-schema#> .
@prefix foaf:	<http://xmlns.com/foaf/0.1/> .

<http://parliament.uk/ontologies/procedure/> 
    rdf:type owl:Ontology ;
    dcterms:title "Procedure ontology"@en ;
    dcterms:created "2018-02-20"^^xsd:date ;
	dcterms:rights "Open Parliament Licence v3.0"@en ;
    dcterms:description "An abstract ontology for describing how process steps can be combined to form a procedure. In this model, the procedure is analogous to a journey map to a set of potential destinations, a route is a set of directions on one of those journeys and a step is a waypoint."@en ;
	foaf:depiction <https://ukparliament.github.io/ontologies/procedure/procedure.png> ;
	foaf:maker
		[ foaf:name "Chris Alcock" ],
		[ foaf:name "David Beamish" ],
		[ foaf:name "Robert Brook"; foaf:homepage <https://robert-brook.com/> ],
		[ foaf:name "Gordon Clarke" ],
		[ foaf:name "Jack Dent" ],
		[ foaf:name "Samu Lang" ],
		[ foaf:name "Silver Oliver" ],
		[ foaf:name "Michael Smethurst"; foaf:homepage <http://smethur.st/> ],
	    [ foaf:name "Anya Somerville" ],
	    [ foaf:name "Dominic Stockbridge" ],
	    [ foaf:name "Jayne Sunley" ],
		[ foaf:name "James Vinter" ],
		[ foaf:name "Jane White" ],
		[ foaf:name "Ben Woodhams" ].


#######  Classes #####
	
ppr:Procedure rdf:type owl:Class ;
	rdfs:label "Procedure"@en ;
	rdfs:comment "A procedure in a House or Houses. For example, the passage of a made affirmative statutory instrument in both Houses. A procedure may consist of business in a particular House, such as a division; business undertaken by both Houses jointly, such as a joint committee; processes applying to either House, such as a time period; and activities outside Parliament, such as the making of a statutory instrument. In this model a procedure that consists of business in both Houses is considered as a single procedure. Procedures may be constructed from commonly occurring sets of routes. For example, the set of routes involved in EVEL certification."@en ;
	rdfs:isDefinedBy <http://parliament.uk/ontologies/procedure/> .
	
ppr:Route rdf:type owl:Class ;
	rdfs:label "Route"@en ;
	rdfs:comment "A route is a link from one step to another. The source of a route may also be its destination. A route is available when the from step is True, actualised by a business item having a date in the past, or by the input from a logic gate step being True. The validity period of a route may be indicated by its start or end date. A route linking a business step actualised by a business item with a date in the past to a business step which has not been actualised indicates that actualisation of the step will happen in the future, being a causal relationship."@en ;
	rdfs:isDefinedBy <http://parliament.uk/ontologies/procedure/> .

ppr:Step rdf:type owl:Class ;
	rdfs:label "Step"@en ;
	rdfs:comment "A step is either a business step, a logic gate step or a decision step. Steps are joined by routes to form procedures. For example, within the SI procedures there exists a step named 'English Votes for English Laws (EVEL) consideration'. Steps may occur in more than one procedure. For example, all statutory instrument procedures include the EVEL consideration step."@en ;
	rdfs:isDefinedBy <http://parliament.uk/ontologies/procedure/> .

ppr:LogicGateStep rdf:type owl:Class ;
	rdfs:subClassOf ppr:Step ;
	rdfs:label "Logic gate step"@en ;
	rdfs:comment "A logic gate step performs a logical operation on one or more routes. Both the input and the output of a logic gate are either True or False. A route linking a business step actualised by a business item with a date in the past to a business step which has not been actualised by means of a logic gate step with type NOT indicates that actualisation of the step cannot happen in the future, being a precluding relationship. A step may preclude itself from repeated actualisations by means of a set of routes through a logic gate step of type NOT to itself. For example, in the made affirmative statutory instrument procedure the step 'cleared by the Joint Committee on Statutory Instruments' may happen only once, being a precluding relationship."@en ;
	rdfs:isDefinedBy <http://parliament.uk/ontologies/procedure/> .
	
ppr:LogicGateType rdf:type owl:Class ;
	rdfs:label "Logic gate type"@en ;
	rdfs:comment "A logic gate has a type of NOT, AND or OR. A logic gate with type NOT when given True has the result False and when given False has the result True. A logic gate with type AND takes at least two routes as inputs: if all are True the output route is True. A logic gate with type OR takes at least two routes as inputs: if at least one is True the output route is True."@en ;
	rdfs:isDefinedBy <http://parliament.uk/ontologies/procedure/> .
	
ppr:DecisionStep rdf:type owl:Class ;
	rdfs:subClassOf ppr:Step ;
	rdfs:label "Decision step"@en ;
	rdfs:comment "A decision step describes the requirement for a decision to be made before the to route can be followed. Routes may be indicated as allowed rather than causal by means of a decision step. A route linking a business step actualised by a business item with a date in the past to a business step which has not been actualised by means of a decision step indicates that actualisation of the step may happen in the future, being an allowed relationship."@en ;
	rdfs:isDefinedBy <http://parliament.uk/ontologies/procedure/> .
	
ppr:BusinessStep rdf:type owl:Class ;
	rdfs:subClassOf ppr:Step ;
	rdfs:label "Business step"@en ;
	rdfs:comment "A business step is a step that can be actualised by a business item."@en ;
	rdfs:isDefinedBy <http://parliament.uk/ontologies/procedure/> .
	
ppr:House rdf:type owl:Class ;
	rdfs:label "House"@en ;
	rdfs:comment "A House forming part of a parliament. For example, the House of Lords."@en ;
	rdfs:isDefinedBy <http://parliament.uk/ontologies/procedure/> .
	
ppr:BusinessItem rdf:type owl:Class ;
	rdfs:label "Business item"@en ;
	rdfs:comment "An item of business conducted either within or outside Parliament. For example: a second reading debate, the tabling of an early day motion, a laying of a paper, the making of a statutory instrument by a government minister."@en ;
	rdfs:isDefinedBy <http://parliament.uk/ontologies/procedure/> .
	
ppr:WorkPackage rdf:type owl:Class ;
	rdfs:label "Work package"@en ;
	rdfs:comment "A grouping of business items which may be a group falling under a procedure, or a grouping determined by a committee. For example, business items considered during the passage of a particular statutory instrument or public bill, or during an inquiry by a select committee."@en ;
	rdfs:isDefinedBy <http://parliament.uk/ontologies/procedure/> .
	
ppr:WorkPackageableThing rdf:type owl:Class ;
	rdfs:label "Work packageable thing"@en ;
	rdfs:comment "A thing which is the focus of a work package. For example a statutory instrument paper or the work of a government department."@en ;
	rdfs:isDefinedBy <http://parliament.uk/ontologies/procedure/> .
	


#######  Object properties ##### 

ppr:formsPartOf rdf:type owl:ObjectProperty ;
	rdfs:label "Forms part of"@en ;
	rdfs:comment "Relates a business item to a work package it forms part of. One or more business items may form part of a work package. A business item may form part of one or more work packages. For example, a meeting of the Joint Committee on Statutory Instruments may consider one or more SIs, each SI being the focus of a separate work package."@en ;
	rdfs:domain ppr:BusinessItem ;
	rdfs:range ppr:WorkPackage ;
	rdfs:isDefinedBy <http://parliament.uk/ontologies/procedure/> .

ppr:subjectTo rdf:type owl:ObjectProperty ;
	rdfs:label "Subject to"@en ;
	rdfs:comment "Relates a work package to the procedure it is subject to. A work package is only subject to one procedure."@en ;
	rdfs:domain ppr:WorkPackage ;
	rdfs:range ppr:Procedure ;
	rdfs:isDefinedBy <http://parliament.uk/ontologies/procedure/> .
	
ppr:hasConcludingStep rdf:type owl:ObjectProperty ;
	rdfs:label "Has concluding step"@en ;
	rdfs:comment "A procedure may have one or more steps described as concluding steps, at which a work package subject to that procedure is considered to be concluded."@en ;
	rdfs:domain ppr:Procedure ;
	rdfs:range ppr:BusinessStep ;
	rdfs:isDefinedBy <http://parliament.uk/ontologies/procedure/> .
	
ppr:hasKeyStep rdf:type owl:ObjectProperty ;
	rdfs:label "Has key step"@en ;
	rdfs:comment "A procedure may have one or more business steps described as key steps."@en ;
	rdfs:domain ppr:Procedure ;
	rdfs:range ppr:BusinessStep ;
	rdfs:isDefinedBy <http://parliament.uk/ontologies/procedure/> .
	
ppr:hasMemberActionStep rdf:type owl:ObjectProperty ;
	rdfs:label "Has Member action step"@en ;
	rdfs:comment "A procedure may have one or more steps described as Member action steps, points at which a Member is able to take an action."@en ;
	rdfs:domain ppr:Procedure ;
	rdfs:range ppr:BusinessStep ;
	rdfs:isDefinedBy <http://parliament.uk/ontologies/procedure/> .
	
ppr:actualises rdf:type owl:ObjectProperty ;
	rdfs:label "Actualises"@en ;
	rdfs:comment "Relates a business item to a step in a procedure by means of a route. For example, relating the second reading of a public bill to the second reading step in the procedure. A step may be actualised by more than one business item in different work packages. A business item may actualise one or more steps. For example, a business item appearing in the Order Paper including a debate on several motions may actualise steps relating to each motion."@en ;
	rdfs:domain ppr:BusinessItem ;
	rdfs:range ppr:BusinessStep ;
	rdfs:isDefinedBy <http://parliament.uk/ontologies/procedure/> .

ppr:fromStep rdf:type owl:ObjectProperty ;
	rdfs:label "From step"@en ;
	rdfs:comment "Relates a route to its input step."@en ;
	rdfs:domain ppr:Route ;
	rdfs:range ppr:Step ;
	rdfs:isDefinedBy <http://parliament.uk/ontologies/procedure/> .
	
ppr:toStep rdf:type owl:ObjectProperty ;
	rdfs:label "To step"@en ;
	rdfs:comment "Relates a route to its output step."@en ;
	rdfs:domain ppr:Route ;
	rdfs:range ppr:Step ;
	rdfs:isDefinedBy <http://parliament.uk/ontologies/procedure/> .
	
ppr:hasLogicGateType rdf:type owl:ObjectProperty ;
	rdfs:label "Has logic gate type"@en ;
	rdfs:comment "Relates a logic gate step to a logic gate type. A logic gate step has one type."@en ;
	rdfs:domain ppr:LogicGateStep ;
	rdfs:range ppr:LogicGateType ;
	rdfs:isDefinedBy <http://parliament.uk/ontologies/procedure/> .
	
ppr:followsRoute rdf:type owl:ObjectProperty ;
	rdfs:label "Follows route"@en ;
	rdfs:comment "Relates a procedure to a route. A route may appear in one or more procedures. For example, the route between 'Considered for English votes for English laws (EVEL) certification' to 'Certified as England only under the English votes for English laws (EVEL) process' appears in the draft negative, made negative, draft affirmative and made affirmative procedures."@en ;
	rdfs:domain ppr:Procedure ;
	rdfs:range ppr:Route ;
	rdfs:isDefinedBy <http://parliament.uk/ontologies/procedure/> .
	
ppr:stepInHouse rdf:type owl:ObjectProperty ;
	rdfs:label "Step in House"@en ;
	rdfs:comment "Relates a step to one or both Houses where such a relationship exists. A step may exist with no relationship to a House. For example, the making of a statutory instrument happens outside of Parliament."@en ;
	rdfs:domain ppr:Step ;
	rdfs:range ppr:House ;
	rdfs:isDefinedBy <http://parliament.uk/ontologies/procedure/> .
		
ppr:procedureInHouse rdf:type owl:ObjectProperty ;
	rdfs:label "Procedure in House"@en ;
	rdfs:comment "Relates a procedure to one or both Houses."@en ;
	rdfs:domain ppr:Procedure ;
	rdfs:range ppr:House ;
	rdfs:isDefinedBy <http://parliament.uk/ontologies/procedure/> .
		
ppr:focus rdf:type owl:ObjectProperty ;
	rdfs:label "Focus"@en ;
	rdfs:comment "Relates a work package to its focus, this being a work packageable thing."@en ;
	rdfs:domain ppr:WorkPackage ;
	rdfs:range ppr:WorkPackageableThing ;
	rdfs:isDefinedBy <http://parliament.uk/ontologies/procedure/> .